$$
\hat a_\pm=\frac{1}{\sqrt{2\hbar m\omega}}(\mp i\hat p+m\omega \hat x)
$$
$$
\hat H=\hbar\omega(\hat a_{-} \hat a_{+}-\frac{1}{2})=\hbar\omega(\hat a_{+} \hat a_{-}+\frac{1}{2})
$$
$$
\hat a_+\psi_n=\sqrt{n+1}\psi_{n+1},\quad \hat a_-\psi_n=\sqrt{n}\psi_{n-1}
$$
$$
\hat a_{-}\psi_{0}=0,\quad \psi_0=(\frac{m\omega}{\pi\hbar})^{\frac{1}{4}}e^{-\frac{m\omega}{2\hbar}x^{2}},\quad E_0=\frac{1}{2}\hbar\omega
$$
$$
\psi_n=\frac{1}{\sqrt{n!}}(\hat a_+)^{n}\psi_{0},\quad E_n=(n+\frac{1}{2})\hbar\omega
$$
